Old/TreeParamItrp.v
@@ -1,0 +1,327 @@
+(*
+Inductive TreeFamItrp (G:Ctx) : treeFam->(G->Typ)->Type :=
+	tfItrpUv : TreeFamItrp G Uv (fun g=>typUv) |
+	tfItrpEl p p' : TreeParamItrp G p (fun g=>typUv) p'->
+		TreeFamItrp G (El p) (fun g=>typEl (p' g)) |
+	tfItrpPi A B A' B' : TreeFamItrp G A A'->TreeFamItrp (extCtx G A') B B'->
+		TreeFamItrp G (Pi A B) (fun g=>typPi (A' g) (fun a=>B' (existT A' g a)))
+with TreeParamItrp (G:Ctx) : treeParam->forall T:G->Typ,(forall g,T g)->Type :=
+	tpItrpVar i T (i':AtCtx G i T) : TreeParamItrp G (var i) T (ctxProj i') |
+	tpItrpApl f a B P (a':AtCtx G a P) B' f' :
+		TreeFamItrp (extCtx G P) B B'->
+		TreeParamItrp G f (fun g=>typPi (P g) (fun p=>B' (existT P g p))) f'->
+		TreeParamItrp G (apl f a B) (fun g=>B' (existT P g (ctxProj a' g))) (fun g=>f' g (ctxProj a' g)).
+*)
+
+Inductive TFItrpEl (G:Ctx) (R:forall G (T:_->Typ),(forall g,T g)->Type) : (G->Typ)->Type :=
+	tfItrpEl p' : R G (fun g=>typUv) p'->
+		TFItrpEl G R (fun g=>typEl (p' g)).
+Implicit Arguments tfItrpEl [G R p'].
+
+Inductive TFItrpPi (G:Ctx) (RA RB:forall G:Ctx,(G->Typ)->Type) : (G->Typ)->Type :=
+	tfItrpPi A' B' : RA G A'->RB (extCtx G A') B'->
+		TFItrpPi G RA RB (fun g=>typPi (A' g) (fun a=>B' (existT A' g a))).
+Implicit Arguments tfItrpPi [G RA RB A' B'].
+
+Inductive TPItrpVar (G:Ctx) i : forall T:G->Typ,(forall g,T g)->Type :=
+	tpItrpVar T (i':AtCtx G i T) : TPItrpVar G i T (ctxProj i').
+Implicit Arguments tpItrpVar [G i T].
+
+Inductive TPItrpApl (G:Ctx) (Rf:forall G (T:_->Typ),(forall g,T g)->Type) a (RB:forall G:Ctx,(G->Typ)->Type) :
+forall T:G->Typ,(forall g,T g)->Type :=
+	tpItrpApl P (a':AtCtx G a P) B' f' :
+		RB (extCtx G P) B'->
+		Rf G (fun g=>typPi (P g) (fun p=>B' (existT P g p))) f'->
+		TPItrpApl G Rf a RB (fun g=>B' (existT P g (ctxProj a' g))) (fun g=>f' g (ctxProj a' g)).
+Implicit Arguments tpItrpApl [Rf a RB P B' f'].
+
+Fixpoint TreeFamItrp (G:Ctx) F : (G->Typ)->Type := match F with
+	Uv => eq (fun g=>typUv) |
+	El p => TFItrpEl G (fun G=>TreeParamItrp G p) |
+	Pi A B => TFItrpPi G (fun G=>TreeFamItrp G A) (fun G=>TreeFamItrp G B)
+end
+with TreeParamItrp G p : forall T,_->Type := match p with
+	var i => TPItrpVar G i |
+	apl f a B => TPItrpApl G (fun G=>TreeParamItrp G f) a (fun G=>TreeFamItrp G B)
+end.
+
+----------
+
+Lemma tpItrpBump G n l p GL P (xg:ExtCtx GL l G) : forall T p',TreeParamItrp G (pBump n l p) T p'->
+TreeParamItrp (ctxBump P xg) (pBump (S n) l p) (elBump P xg T) (elBump P xg p').
+	(*induction la;simpl.
+
+	intros.
+	apply spItrpNilInv with (1 := X).
+	apply spItrpNil.
+
+	intros ? ?.
+	destruct (lt_dec a l) as [Ho | Ho].
+		rewrite (proj1 (nat_compare_lt _ _) Ho).
+		intro.
+		apply spItrpConsInv with (1 := X).
+		clear T la' X.
+		intros.
+		pose proof (spItrpCons _ _ _ _ _ _ (atBumpGLo P xg a' Ho)
+			(fun d g=>B d (existT _ (xc_f' (xgBumpG P xg) d (projT1 g)) (projT2 g)))
+			_ (IHla _ _ X)).
+		simpl in X0.
+		rewrite ctxProj_BumpGLo in X0.
+		exact X0.
+
+		assert (nolt : forall k,k = match nat_compare a l with
+			Lt => a |
+			_ => k
+		end).
+			intro.
+			destruct (nat_compare_spec a l);try reflexivity.
+			destruct (Ho H).
+		rewrite <- nolt.
+		rewrite <- nolt.
+		clear nolt.
+		intro.
+		apply spItrpConsInv with (1 := X).
+		clear T la' X.
+		intros.
+		assert (l <= n + a).
+			rewrite <- plus_comm.
+			apply le_plus_trans.
+			exact (not_lt _ _ Ho).
+		pose proof (spItrpCons _ _ _ _ _ _ (atBumpGHi P xg a' H)
+			(fun d g=>B d (existT _ (xc_f' (xgBumpG P xg) d (projT1 g)) (projT2 g)))
+			_ (IHla _ _ X)).
+		simpl in X0.
+		rewrite ctxProj_BumpGHi in X0.
+		exact X0.
+Qed.*)
+Admitted.
+
+Lemma tpItrpBump_O G n p T p' P : TreeParamItrp G (pBump n O p) T p'->
+TreeParamItrp (extCtx G P) (pBump (S n) O p) (fun g=>T (projT1 g)) (fun g=>p' (projT1 g)).
+	apply tpItrpBump with (P := P) (xg := extOCtx G).
+Qed.
+
+Lemma tfItrpBump n F GL P : forall G l F' (xg:ExtCtx GL l G),TreeFamItrp G (fBump n l F) F'->
+TreeFamItrp (ctxBump P xg) (fBump (S n) l F) (elBump P xg F').
+	(*induction F as [| p];[| destruct p as (f,la)];simpl;intros.
+
+	rewrite sfItrpNilInv with (1 := X).
+	apply sfItrpNil.
+
+	apply sfItrpConsInv with (1 := X).
+	clear F' X.
+	intros B ? ? F'.
+	pose (A d g := la' d g (tctxProj f' d)).
+	change (forall d,extCtx G A d->Type) in F'.
+	pose (F_ d g := forall p,F' d (existT _ g p)).
+	change (SimpParamItrp G B (laBumpG n l la) (fun d g=>Type) la'->
+		SimpFamItrp D (extCtx G A) (fBumpG n (S l) F) F'->
+		SimpFamItrp D (ctxBumpG P xg) ((f,laBumpG (S n) l la) :: fBumpG (S n) (S l) F) (elBumpG P xg F_)).
+	intros Xp Xf.
+	apply sfItrpCons with (la' := elBumpG P xg la') (2 := IHF _ _ _ (extSCtx xg _) Xf).
+	apply spItrpBumpG with (1 := Xp) (xg := xg).
+Qed.*)
+Admitted.
+
+Lemma tfItrpBump_O G n F F' P : TreeFamItrp G (fBump n O F) F'->
+TreeFamItrp (extCtx G P) (fBump (S n) O F) (fun g=>F' (projT1 g)).
+	apply tfItrpBump with (P := P) (xg := extOCtx G).
+Qed.
+
+Lemma tpItrpSubst G p l b GL P (xg:ExtCtx (extCtx GL P) l G) (b':AtCtx GL b P) : forall T p',
+	TreeParamItrp G p T p'->
+TreeParamItrp (ctxSubst xg (ctxProj b')) (pSubst l b p)
+(elSubst xg T (ctxProj b')) (elSubst xg p' (ctxProj b')).
+	(*induction la;intros ? ?;simpl.
+
+	intro.
+	apply spItrpNilInv with (1 := X).
+	apply spItrpNil.
+
+	destruct (lt_eq_lt_dec a l) as [s | Ho];[destruct s as [Ho | Ho] |].
+		intro.
+		rewrite (proj1 (nat_compare_lt _ _) Ho).
+		apply spItrpConsInv with (1 := X).
+		clear T la' X.
+		intros.
+		pose proof (spItrpCons _ _ _ _ _ _ (atSubstLt xg a' Ho (ctxProj b'))
+			(fun d g=>B d (existT _ (xc_f' (xgSubst xg (ctxProj b')) d (projT1 g)) (projT2 g)))
+			_ (IHla _ _ X)).
+		simpl in X0.
+		rewrite ctxProj_SubstLt in X0.
+		exact X0.
+
+		intro.
+		rewrite (proj2 (nat_compare_eq_iff _ _) Ho).
+		revert xg IHla.
+		apply (tr (fun _=>_) Ho).
+		clear l Ho.
+		intros.
+		apply spItrpConsInv with (1 := X).
+		clear T la' X.
+		intros.
+		pose (b0 := tr (AtCtx G _) (atCtxExtTEq b' xg a') (ax_a (atCtxExt xg (popCtx b' P)))).
+		assert (Ha : a + S b = S (a + b)).
+			rewrite <- plus_n_Sm.
+			reflexivity.
+		pose (b1 := tr (fun n=>AtCtx G n P0) Ha b0).
+		simpl in b1.
+		assert (Hb : a <= a + b).
+			apply le_plus_l.
+		pose proof (spItrpCons _ _ _ _ _ _ (atSubstGt xg b1 Hb (ctxProj b'))
+			(fun d g=>B d (existT _ (xc_f' (xgSubst xg (ctxProj b')) d (projT1 g)) (projT2 g)))
+			_ (IHla _ _ X)).
+		simpl in X0.
+		rewrite ctxProj_SubstGt in X0.
+		subst b1.
+		rewrite <- Ha in X0.
+		simpl in X0.
+		clear Ha Hb.
+		subst b0.
+		rewrite ctxProj_Ext in X0.
+		rewrite ctxProj_SubstEq in X0.
+		exact X0.
+
+		rewrite (proj1 (nat_compare_gt _ _) Ho).
+		destruct a.
+			exact (match lt_n_O _ Ho with end).
+		unfold lt in Ho.
+		intro.
+		simpl.
+		apply spItrpConsInv with (1 := X).
+		clear T la' X.
+		intros.
+		pose proof (le_S_n _ _ Ho).
+		pose proof (spItrpCons _ _ _ _ _ _ (atSubstGt xg a' H (ctxProj b'))
+			(fun d g=>B d (existT _ (xc_f' (xgSubst xg (ctxProj b')) d (projT1 g)) (projT2 g)))
+			_ (IHla _ _ X)).
+		simpl in X0.
+		rewrite ctxProj_SubstGt in X0.
+		exact X0.
+Qed.*)
+Admitted.
+
+Lemma tpItrpSubst_O G P p b T p' (b':AtCtx G b P) : TreeParamItrp (extCtx G P) p T p'->
+TreeParamItrp G (pSubst O b p) _ (fun g=>p' (existT _ g (ctxProj b' g))).
+	apply tpItrpSubst with (xg := extOCtx (extCtx G P)) (b' := b').
+Qed.
+
+Lemma tfItrpSubst F b GL P (b':AtCtx GL b P) : forall G l F' (xg:ExtCtx (extCtx GL P) l G),TreeFamItrp G F F'->
+TreeFamItrp (ctxSubst xg (ctxProj b')) (fSubst l b F) (elSubst xg F' (ctxProj b')).
+	(*induction F as [| p];[| destruct p as (f,la)];simpl;intros.
+
+	rewrite sfItrpNilInv with (1 := X).
+	apply sfItrpNil.
+
+	apply sfItrpConsInv with (1 := X).
+	clear F' X.
+	intros B ? ? F'.
+	pose (A d g := la' d g (tctxProj f' d)).
+	change (forall d,extCtx G A d->Type) in F'.
+	pose (F_ d g := forall p,F' d (existT _ g p)).
+	change (SimpParamItrp G B la (fun d g=>Type) la'->
+		SimpFamItrp D (extCtx G A) F F'->
+		SimpFamItrp D (ctxSubst xg (ctxProj b')) ((f,laSubstG la l b) :: fSubstG F (S l) b)
+			(elSubst xg F_ (ctxProj b'))).
+	intros Xp Xf.
+	apply sfItrpCons with (la' := elSubst xg la' (ctxProj b')) (2 := IHF _ _ _ (extSCtx xg _) Xf).
+	apply spItrpSubst with (1 := Xp) (xg := xg).
+Qed.*)
+Admitted.
+
+Lemma tfItrpSubst_O G P F b F' (b':AtCtx G b P) : TreeFamItrp (extCtx G P) F F'->
+TreeFamItrp G (fSubst O b F) (fun g=>F' (existT _ g (ctxProj b' g))).
+	apply tfItrpSubst with (xg := extOCtx (extCtx G P)) (b' := b').
+Qed.
+
+Lemma tcItrpProj i C : forall G G',(ltd i (length G))->TreeCtxItrp G G'->
+	(forall F,AtCtx G' i F->TreeFamItrp G' (fBump (S i) O (nth i G Uv)) F->C)->
+C.
+	induction i;intros ? ?;(destruct G as [| F];intro;[destruct H |]);simpl;intro;
+	destruct X;intro rtn.
+
+	apply (rtn _ (topCtx G' F')).
+	apply tfItrpBump_O.
+	rewrite fBump_O.
+	exact t0.
+
+	apply (IHi _ _ H t).
+	intros.
+	apply (rtn _ (popCtx X F')).
+	apply tfItrpBump_O.
+	exact X0.
+Qed.
+
+Inductive ExTreeParamItrp G p T : Type :=
+	exTreeParamItrp T' p' : TreeParamItrp G p T' p'->TreeFamItrp G T T'->ExTreeParamItrp G p T.
+Implicit Arguments exTreeParamItrp [G p T].
+
+Lemma tfItrpTotalNest G F C : TreeFamGood
+	(fun G p T=>forall G',TreeCtxItrp G G'->ExTreeParamItrp G' p T) G F->
+forall G',TreeCtxItrp G G'->
+	(forall F',TreeFamItrp G' F F'->C)->
+C.
+	intro.
+	induction X;intros ? XG rtn.
+
+	apply (rtn (fun g=>typUv)).
+	reflexivity.
+
+	destruct (p0 _ XG) as (?,?,Xp,XU).
+	simpl in XU.
+	revert p' Xp.
+	rewrite <- XU.
+	clear T' XU.
+	intros.
+	apply (rtn (fun g=>typEl (p' g))).
+	simpl.
+	exact (tfItrpEl Xp).
+
+	clear X1 X2.
+	apply (IHX1 _ XG).
+	intros A' XA.
+	apply (IHX2 (extCtx G' A')).
+		simpl.
+		exact (tcItrpCons XG XA).
+	intros B' XB.
+	apply (rtn (fun g=>typPi (A' g) (fun a=>B' (existT _ g a)))).
+	simpl.
+	exact (tfItrpPi XA XB).
+Qed.
+
+Lemma tpItrpTotal G p T : TreeParamGood G p T->forall G',TreeCtxItrp G G'->ExTreeParamItrp G' p T.
+	intro.
+	induction H;intros ? XG.
+
+	apply tcItrpProj with (i := i) (2 := XG).
+		unfold ltd.
+		rewrite (proj1 (nat_compare_lt _ _) H).
+		exact I.
+	intros T i' XT.
+	apply (exTreeParamItrp T (ctxProj i')).
+		apply tpItrpVar.
+
+		exact XT.
+
+	apply tcItrpProj with (i := a) (2 := XG).
+		unfold ltd.
+		rewrite (proj1 (nat_compare_lt _ _) H).
+		exact I.
+	intros P a' XP.
+	destruct (IHTreeParamGood _ XG) as (T,f',Xf,XT).
+	simpl in XT.
+	revert f' Xf.
+	destruct XT as (P0,B'0,XP0,XB0).
+	simpl.
+	intros.
+	apply tfItrpTotalNest with (1 := X) (G' := extCtx G' P).
+		simpl.
+		exact (tcItrpCons XG XP).
+	clear X.
+	intros B' XB.
+	(* Aaaaaand we're screwed *)
+	apply (exSimpParamItrp (fun g=>B' (existT _ g (ctxProj a' g))) (fun g f=>la'
+		apply spItrpCons with (a' := a') (1 := Xp).
+
+		apply sfItrpSubst_O with (1 := Xf).
+Qed.
